ProjectEulerSolutions/P47.lean
@@ -43,8 +43,9 @@ example : firstConsecutiveWithKFactors 3 3 2000 = 644 := by
   native_decide
 
 
-def solve (_n : Nat) :=
-  firstConsecutiveWithKFactors 4 4 200000
+def solve (n : Nat) :=
+  let _ := ProjectEulerStatements.P47.exists_consecutive_with_n_factors n
+  firstConsecutiveWithKFactors n n (n + 10)
 
-theorem equiv (n : Nat) : ProjectEulerStatements.P47.naive n n n = solve n := sorry
+theorem equiv (n : Nat) : ProjectEulerStatements.P47.naive n = solve n := sorry
 end ProjectEulerSolutions.P47
