solvers/30.lean
@@ -3,4 +3,4 @@ import ProjectEulerSolutions.P30
 open ProjectEulerSolutions.P30
 
 def main : IO Unit := do
-  IO.println (solve 0)
+  IO.println (solve 5)
